templates/lockfree/skiplist_search.v
@@ -11,41 +11,53 @@ From iris.heap_lang.lib Require Import nondet_bool.
 From iris.bi.lib Require Import fractional.
 Set Default Proof Using "All".
 From iris.bi.lib Require Import fractional.
+Require Import skiplist_util.
 Require Export traverse_spec_module flows.
   
   Export skiplist_util.TR.NODE skiplist_util.SK skiplist_util.DEFS.
 
-  Lemma searchOp_spec (Σ : gFunctors) (H' : heapGS Σ) (H'' : dsG Σ) (H''' : hsG Σ)
-    N γ_t γ_r γ_m γ_mt γ_msy r (p: proph_id) pvs tid t0 Q k (hd tl: Node) :
-      main_inv Σ H' H'' H''' N γ_t γ_r γ_m γ_mt γ_msy r -∗
-      thread_start Σ H' H'' H''' γ_t γ_mt tid t0 -∗
-      □ update_helping_protocol Σ H' H'' H''' N γ_t γ_r γ_mt γ_msy -∗
+  Lemma searchOp_spec Σ Hg1 Hg2 Hg3 N γ_t γ_r γ_m γ_mt γ_msy r (p: proph_id) 
+    pvs tid t0 Q k (hd tl: Node) :
+      main_inv Σ Hg1 Hg2 Hg3 N γ_t γ_r γ_m γ_mt γ_msy r -∗
+      thread_start Σ Hg1 Hg2 Hg3 γ_t γ_mt tid t0 -∗
+      □ update_helping_protocol Σ Hg1 Hg2 Hg3 N γ_t γ_r γ_mt γ_msy -∗
       ⌜local_pre (searchOp k)⌝ -∗
+      r ↦□ (#hd, #tl) -∗
         {{{ proph p pvs ∗ 
             (match process_proph tid pvs with
-              contra => au Σ H' H'' H''' N γ_r (searchOp k) Q
+              contra => au Σ Hg1 Hg2 Hg3 N γ_r (searchOp k) Q
             | no_upd => True
-            | upd => au Σ H' H'' H''' N γ_r (searchOp k) Q end) }}}
+            | upd => au Σ Hg1 Hg2 Hg3 N γ_r (searchOp k) Q end) }}}
               search #hd #tl #k @ ⊤
         {{{ (res: resT) prf pvs', RET #res;
             proph p pvs' ∗ ⌜pvs = prf ++ pvs'⌝ ∗
             (match process_proph tid pvs with
               contra => ⌜Forall (λ x, x.2 ≠ #tid) prf⌝
-            | no_upd => past_lin_witness Σ H' H'' H''' γ_m (searchOp k) res t0
+            | no_upd => past_lin_witness Σ Hg1 Hg2 Hg3 γ_m (searchOp k) res t0
             | upd => Q #res ∨ 
                 ⌜Forall (λ x, ¬ is_snd true x ∧ x.2 ≠ #tid) prf⌝ end) }}}.
   Proof. 
-    iIntros "#HInv #Thd_st #Upd [%HL %Range_k]". 
+    iIntros "#HInv #Thd_st #Upd [%HL %Range_k] #HR'". 
     iIntros (Φ) "!# (Hproph & Hmatch) Hpost".
     wp_lam. wp_pures.
-    wp_apply (traverse_spec Σ H' H'' H'''); try done.
+    wp_apply traverse_spec; try done.
     iIntros (preds succs ps ss res) "(Hpreds & Hsuccs & %Len_ps 
       & %Len_ss & %HpsL & %HssL & #Htr)".  
     wp_pures. 
+    iInv "HInv" as (M0 T0 s0) "(>Ds & >%Habs0 & >Hist & Help & >Templ)".
+    iDestruct "Templ" as (hd' tl')"(HR & SShot0 & Res & %PT0 & %Trans_M0)".
+    iAssert (⌜hd' = hd ∧ tl' = tl⌝)%I with "[HR]" as %[-> ->]. 
+    { iDestruct (mapsto_agree with "[$HR] [$HR']") as %[=]. by iPureIntro. }  
     iAssert (past_lin_witness _ _ _ _ γ_m (searchOp k) res t0)%I as "#PastW".
-    { iDestruct "Htr" as "(_ & Htr)". destruct res.
-      all: iDestruct "Htr" as (s)"(#Past_s & %Hk_s & _)".
-      all: iExists s; iFrame "#"; iPureIntro. all: set_solver. }
+    { iDestruct "Htr" as "(_ & Htr)". 
+      iDestruct "Htr" as (s)"(#Past_s & %H')". 
+      set c := ss !!! 0. rewrite -/c in H'.
+      iPoseProof (per_tick_past with "[%] Hist Past_s") as "%PT_s"; try done.
+      iExists s. iFrame "#". iPureIntro. rewrite /seq_spec. split. done.
+      destruct H' as (H' & H'' & H'''). destruct PT_s as (_&_&PT&_).
+      pose proof PT c k H' H'' as H1'. destruct res; set_solver. }
+    iModIntro. iSplitR "Hproph Hmatch Hpost".
+    { iNext. iExists M0, T0, s0. iFrame "∗%". iExists hd, tl. iFrame "∗%". }
     destruct (process_proph tid pvs) eqn: Hpvs.
     - iApply ("Hpost" $! res [] pvs). iFrame "Hproph". by iPureIntro.
     - iApply ("Hpost" $! res [] pvs). iFrame "Hproph". iSplitR. by iPureIntro.
